\startchapter{Least Squares Localization by Sequential Convex Relaxation}
\label{chapter:socp}

%\textbf{Notes for further development.}
%
%2-step approach:
%
%1) identify outliers to reduce the error-prone data points
%
%2) apply the algorithm  to the redused data set
%
%Projection onto convex sets and projection onto rings \textit{cite GhStr}

\section{Second Order Cone Programming}

\section{Range-based localization}

Problem:
Given sensor array ${\Ba_i, i = 1, 2, ..., m}$ and noisey range measurements $r_i$ find the true \textit{unknown} location of $\Bx$ as 
\begin{equation} % 5.1
\Min \sum^m_i \left( \|\Bx - \Ba_i\| - r_i \right)^2 
\end{equation}
which can be (equivalently) written as 
\begin{eqnarray} %5.2
\Min_{\Bx, \Bz} \sum^m_i \left( z_i - r_i \right)^2 \\
\setcounter{equation}{2}
\mbox{subject to: } \|\Bx - \Ba_i\| = z_i, i = 1, 2, ..., m
\end{eqnarray}
The constraint in 5.2 is hard to suffice, therefore we allow a relaxation:
\begin{eqnarray} %5.3
\Min_{\Bx, \Bz} \sum^m_i \left( z_i - r_i \right)^2 \\
\setcounter{equation}{3}
\mbox{subject to: } \|\Bx - \Ba_i\| \leq (1+ \gamma)z_i  \\
\setcounter{equation}{3}
\|\Bx - \Ba_i\| \geq (1 - \gamma)z_i, \quad i = 1, 2, ..., m
\end{eqnarray}
where $\gamma$ is small, typically $0 < \gamma < 0.5$.
This would yield an approximate solution to 5.2 and therefore to 5.1. 
By allowing $\gamma$ to sequentially/monotonically decrease from some small $0 < \gamma_0 < 0.5$ to 0 solution of 5.3 will converge to 5.2.
\textit{Proof} Let $\gamma(k)$ be monotonically decteasing, where $k$ is an iteration count and $0 < \gamma_0 < 0.5$. Then 
$\lim_{\gamma \rightarrow 0} (1 + \gamma)z_i = z_i$ and $\lim_{\gamma \rightarrow 0} (1 - \gamma)z_i = z_i$. Therefore as $\gamma$ approaches 0, the feasible region of the problem in 5.3 will become equivalent to that in 5.2.
As iterations proceed, the objective in 5.3 will not be monotonically decreasing but it will converge to the critical point.

Problem in 5.3 is nonconvex due to nonconvexity of one of its inequality constraint. The constraint in 5.3b $\|\Bx - \Ba_i\| \leq (1+ \gamma)z_i$ is convex, the constraint in 5.3c is not, because
\begin{equation}
\nonumber
\|\Bx - \Ba_i\| \geq (1 - \gamma)z_i \Longleftrightarrow \underbrace{-\|\Bx - \Ba_i\|}_{nonconvex} \leq -(1 - \gamma)z_i
\end{equation}
From convexity of the norm $\|\Bx - \Ba_i\|$ it follows that for some \textit{known} $\Bx_k$
\begin{equation}
\nonumber
\|\Bx - \Ba_i\| \geq \|\Bx_k - \Ba_i\| + \partial\|\Bx_k - \Ba_i\|^T(\Bx - \Ba_i)
\end{equation}
Hence the constraint in 5.3c can be convexified by replacing it with its affine approximation
\begin{equation}
\nonumber
-\|\Bx_k - \Ba_i\| - \partial\|\Bx_k - \Ba_i\|^T(\Bx - \Ba_i) \leq -(1 - \gamma)z_i
\end{equation}
At the $k$th iteration when the iterate $\Bx_k$ is known, the nonconvex problem in 5.3 can be relaxed to an SOCP problem
\begin{eqnarray} %5.4
\Min_{\Bx, \Bz} \sum^m_i \left( z_i - r_i \right)^2 \\
\setcounter{equation}{4}
\mbox{subject to: } \|\Bx - \Ba_i\| \leq (1+ \gamma)z_i  \\
\setcounter{equation}{4}
-\|\Bx_k - \Ba_i\| - \partial\|\Bx_k - \Ba_i\|^T(\Bx - \Ba_i) \leq -(1 - \gamma)z_i \\
\nonumber
\quad i = 1, 2, ..., m
\end{eqnarray}

The relaxation parameter $\gamma$ controls the size of the convex hull that defines a feasibility region of the problem 5.4.
$\gamma$ needs to be monotonically decreasing with increase of the iteration count. Start with some $0 < \gamma_0 < 0.5$, typically $\gamma0 = 0.3$ or 0.2 is good. After $k$th iteration update $\gamma_{k+1}$ linearly as
\begin{equation}
\nonumber
\gamma_{k+1} = \gamma_0 - k\frac{\gamma_0}{K_{max} - 1}
\end{equation}
or quadratically as
\begin{equation}
\nonumber
\gamma_{k+1} = \gamma_0\frac{(K_{max} - 1 - k)^2}{(K_{max} - 1)^2}
\end{equation}


%\startchapter{SOCP}

\section{Range-Difference Localization}

Measurement model
\begin{equation} \label{eq:6.1}
d_i = \|\Bx - \Ba_i\| - \|\Bx\| + noise
\end{equation}

Least-squares formulation
\begin{equation} \label{eq:6.2}
\Min \sum^m_{i=1}\left( \|\Bx - \Ba_i\| - \|\Bx\| - d_i\right)^2
\end{equation}
The problem in 6.2 can be equivalently written as
\begin{eqnarray} \label{eq:6.3}
\Min \sum^m_{i=1}\left( z_i - y - d_i\right)^2\\
\nonumber
\mbox{subject to: } \|\Bx - \Ba_i\| = z_i \\
\nonumber
\|\Bx\| = y \\
\nonumber
z_i \geq 0, \ y \geq 0
\\ \nonumber  i = 1, 2, \ldots m
\end{eqnarray}

Let $\tilde{\Bx} = [\Bx^T \ y \ z_1 \ldots z_m]^T$, $\tilde{\Bx} \in R^{m+n+1}$ be a known feasible point of the problem in 6.3 and $\Bdelta_{\tilde{\Bx}} = [\Bdelta_x^T \  \delta_y \ \delta_{z_1} \ \ldots \  \delta_{z_m}]^T$ a small perturbation to it, such that $|\Bdelta_{\tilde{\Bx}}| \leq \beta$, and $\beta > 0$ is a small positive constant. At the $k$th iterations with $\tilde{\Bx}^k$ \textit{known} update $(\Bx^k, y^k, \Bz^k)$ to 
\begin{eqnarray} \label{eq:6.4}
\Bx^{k+1} = \Bx^k + \Bdelta_x \\
\nonumber
y^{k+1} = y^k + \delta_y \\
\nonumber
\Bz^{k+1} = \Bz^k + \Bdelta_z
\end{eqnarray}
Substituting 6.4 in 6.3 the objective in 6.3a cam be written as
\begin{eqnarray} \label{eq:6.5}
F(\hat{\Bx}) & =  & \sum^m_{i = 1} \left(z^k_i + \delta_{z_i} - (y^k + \delta_y) - d_i \right)^2 \\
\nonumber
& = & \sum^m_{i = 1} \left(- \delta_y + \delta_{z_i}  - \tilde{d_i} \right)^2
\end{eqnarray}
where $\tilde{d_i} = y^k - z_i^k + d_i$ are grouped known constant terms.
Substituting 6.4b in 6.3b
\begin{equation}
\nonumber
\|\Bx^k + \Bdelta^k_x - \Ba_i\| = z^k_i +\delta_{z_i}, \quad i = 1, 2, \ldots, m
\end{equation}
Re-grouping the terms on the left side of the equality and squaring both sides 
\begin{eqnarray}
\nonumber
\|(\Bx^k  - \Ba_i) + \Bdelta^k_x\|^2 & = & \left(z^k_i +\delta_{z_i}\right)^2 \\
\nonumber
\Leftrightarrow 
\|\Bx^k  - \Ba_i\|^2 + 2\left( \Bx^k  - \Ba_i \right)^T\Bdelta_x + \cancelto{\mbox{\scriptsize{small}}}{\|\Bdelta_x\|^2}  & = & \left(z_i^k\right)^2 + 2z_i^k\delta_{z_i} + \cancelto{\mbox{\scriptsize{small}}}{\Bdelta^2_{z_i}} \\
\nonumber
\Leftrightarrow \|\Bx^k  - \Ba_i\|^2 + 2\left( \Bx^k  - \Ba_i \right)^T\Bdelta_x   & \approx & \left(z_i^k\right)^2 + 2z_i^k\delta_{z_i} \\
\nonumber
\Leftrightarrow \|\Bx^k  - \Ba_i\|^2 + 2\left( \Bx^k  - \Ba_i \right)^T\Bdelta_x   & \approx & \left(z_i^k\right)^2 + 2z_i^k\delta_{z_i} \\
\nonumber
- 2\left( \Bx^k  - \Ba_i \right)^T\Bdelta_x + 2z_i^k\delta_{z_i}  & \approx & \|\Bx^k  - \Ba_i\|^2 - \left(z_i^k\right)^2
\end{eqnarray}
Repeating the similar procedure with the constraint in 6.3c
\begin{eqnarray}
\nonumber
\|\Bx^k + \Bdelta_x\| & = & y^k + \delta_y \\
\nonumber
\|\Bx^k + \Bdelta_x\|^2 & = & \left(y^k + \delta_y \right)^2 \\
\nonumber
\Leftrightarrow \|\Bx^k\|^2 + 2\Bdelta_x^T\Bx^k + \cancelto{\mbox{\scriptsize{small}}}{\|\Bdelta_x\|^2} & = & \left(y^k\right)^2 + 2y^k\delta_y +  \cancelto{\mbox{\scriptsize{small}}}{\delta_y^2} \\
\nonumber
\Leftrightarrow -2\left(\Bx^k\right)^T\delta_x + 2y^k\delta & \approx & \|\Bx\|^2 - \left(y^k\right)^2
\end{eqnarray}
The problem in 6.3 can now be written in terms of the \textit{known} feasible  iterate $\tilde{\Bx}$ and its \textit{unknown} perturbation  $\Bdelta_{\tilde{\Bx}}$ as
\begin{eqnarray} \label{eq:6.6}
\Min_{\tilde{\Bx}, \Bdelta_{\tilde{\Bx}}} \sum^m_{i=1}\left( -\delta_y + \delta_{z_i} -\tilde{d_i}\right)^2\\
\nonumber
\mbox{subject to: } \Leftrightarrow -2\left(\Bx^k\right)^T\delta_x + 2y^k\delta = \|\Bx\|^2 - \left(y^k\right)^2 \\
\nonumber
-2\left(\Bx^k\right)^T\delta_x + 2y^k\delta = \|\Bx\|^2 - \left(y^k\right)^2 \\
\nonumber
|\Bdelta_{\tilde{\Bx}}|  \leq \beta \\
\nonumber
z_i^k + \delta_{z_i} \geq 0, \ 
y^k + \delta_y \geq 0
\\ \nonumber  i = 1, 2, \ldots m
\end{eqnarray}
where $\tilde{d_i} = y^k - z_i^k + d_i$. 
The constraint $\beta$ was imposed on each element of the vector $\Bdelta_{\tilde{\Bx}}$ to guarantee that at each iteration is sufficiently small.
The iterate $\tilde{\Bx}^k$ is feasible and known but it is not guaranteed that the $\tilde{\Bx}^{k+1}$ will also be feasible. To allow non-feasible perturbations $\Bdelta_{\tilde{\Bx}}$, the problem can be overcome by introducing a
nonnegative slack variable $s \geq 0$ 6.6c to replace their right-hand sides  by a  relaxed upper bound (as this new bound itself is a nonnegative variable). This leads to a following formulation of the problem in 6.3
\begin{eqnarray} \label{eq:6.7}
\Min_{s, \tilde{\Bx}, \Bdelta_{\tilde{\Bx}}} \sum^m_{i=1}\left( -\delta_y + \delta_{z_i} -\tilde{d_i}\right)^2 + \mu s \\
\nonumber
\mbox{subject to: }  -2\left(\Bx^k\right)^T\delta_x + 2y^k\delta = \|\Bx\|^2 - \left(y^k\right)^2 \\
\nonumber
-2\left(\Bx^k\right)^T\delta_x + 2y^k\delta = \|\Bx\|^2 - \left(y^k\right)^2 \\
\nonumber
|\Bdelta_{\tilde{\Bx}}|  \leq \beta + s\\
\nonumber
s \geq 0 \\ 
\nonumber
z_i^k + \delta_{z_i} \geq 0, \ 
y^k + \delta_y \geq 0
\\ \nonumber  i = 1, 2, \ldots m
\end{eqnarray}
